de bruijn tests

translations/param_unary.v
@@ -8,6 +8,10 @@ Local Infix "<=" := Nat.leb.
 Definition default_term := tVar "constant_not_found".
 Definition debug_term msg:= tVar ("debug: " ^ msg).
 
+
+
+
+
 (* lifts everything after n *)
 (* morally identity *)
 (* TODO: general nested lifting *)
@@ -29,6 +33,98 @@ Fixpoint tsl_rec0 (n : nat) (t : term) {struct t} : term :=
   | _ => t
   end.
 
+Definition tsl_rec0' (n : nat) (t : term) : term := t.
+
+
+Definition subst_app := mkApps.
+
+
+Fixpoint tsl_rec1_app (app : option term) (E : tsl_table) (t : term) : term :=
+  let tsl_rec1 := tsl_rec1_app None in
+  let debug case symbol :=
+      debug_term ("tsl_rec1: " ^ case ^ " " ^ symbol ^ " not found") in
+  match t with
+  | tLambda na A t =>
+    let A0 := tsl_rec0 0 A in
+    let A1 := tsl_rec1_app None E A in
+    tLambda na A0 (tLambda (tsl_name tsl_ident na)
+                           (subst_app (lift0 1 A1) [tRel 0])
+                           (tsl_rec1_app (option_map (lift 2 2) app) E t))
+  | t => let t1 :=
+  match t with
+  | tRel k => tRel (2 * k)
+  | tSort s => tLambda (nNamed "A") (tSort s) (tProd nAnon (tRel 0) (tSort s))
+
+  | tProd na A B =>
+    let A0 := tsl_rec0 0 A in
+    let A1 := tsl_rec1 E A in
+    let B0 := tsl_rec0 1 B in
+    let B1 := tsl_rec1 E B in
+    let ΠAB0 := tProd na A0 B0 in
+    tLambda (nNamed "f") ΠAB0
+      (tProd na (lift0 1 A0)
+             (tProd (tsl_name tsl_ident na)
+                    (subst_app (lift0 2 A1) [tRel 0])
+                    (subst_app (lift 1 2 B1)
+                               [tApp (tRel 2) [tRel 1]])))
+  | tApp t us =>
+    let us' := concat (map (fun v => [tsl_rec0 0 v; tsl_rec1 E v]) us) in
+    mkApps (tsl_rec1 E t) us'
+
+  | tLetIn na t A u =>
+    let t0 := tsl_rec0 0 t in
+    let t1 := tsl_rec1 E t in
+    let A0 := tsl_rec0 0 A in
+    let A1 := tsl_rec1 E A in
+    let u0 := tsl_rec0 0 u in
+    let u1 := tsl_rec1 E u in
+    tLetIn na t0 A0 (tLetIn (tsl_name tsl_ident na) (lift0 1 t1)
+                            (subst_app (lift0 1 A1) [tRel 0]) u1)
+
+  | tCast t c A => let t0 := tsl_rec0 0 t in
+                  let t1 := tsl_rec1 E t in
+                  let A0 := tsl_rec0 0 A in
+                  let A1 := tsl_rec1 E A in
+                  tCast t1 c (mkApps A1 [tCast t0 c A0]) (* apply_subst ? *)
+
+  | tConst s univs =>
+    match lookup_tsl_table E (ConstRef s) with
+    | Some t => t
+    | None => debug "tConst" (string_of_kername s)
+    end
+  | tInd i univs =>
+    match lookup_tsl_table E (IndRef i) with
+    | Some t => t
+    | None => debug "tInd" (match i with mkInd s _ => string_of_kername s end)
+    end
+  | tConstruct i n univs =>
+    match lookup_tsl_table E (ConstructRef i n) with
+    | Some t => t
+    | None => debug "tConstruct" (match i with mkInd s _ => string_of_kername s end)
+    end
+  | tCase ik t u brs as case =>
+    let brs' := List.map (on_snd (lift0 1)) brs in
+    let case1 := tCase ik (lift0 1 t) (tRel 0) brs' in
+    match lookup_tsl_table E (IndRef (fst ik)) with
+    | Some (tInd i _univ) =>
+      tCase (i, (snd ik) * 2)%nat
+            (tsl_rec1_app (Some (tsl_rec0 0 case1)) E t)
+            (tsl_rec1 E u)
+            (map (on_snd (tsl_rec1 E)) brs)
+    | _ => debug "tCase" (match (fst ik) with mkInd s _ => string_of_kername s end)
+    end
+  | tProj _ _ => todo "tsl"
+  | tFix _ _ | tCoFix _ _ => todo "tsl"
+  | tVar _ | tEvar _ _ => todo "tsl"
+  | tLambda _ _ _ => tVar "impossible"
+  end in
+  match app with Some t' => mkApp t1 (t' {3 := tRel 1} {2 := tRel 0})
+               | None => t1 end
+  end.
+
+
+
+
 (* the unary parametricity translation of an object is
 a relation over the objects *)
 (* X_1 is the unary parametricity translation
@@ -38,7 +134,14 @@ types T are translated into relations of objects of type T
   (using lambas for the objects)
 terms are translated to proofs of the relations
 *)
-Fixpoint tsl_rec1 (E : tsl_table) (t : term) : term :=
+Definition up (relTrans:nat->nat) (n:nat) :nat :=
+  pred (relTrans n).
+  (* match n with
+  1 => O
+  | _ => n
+  end. *)
+
+Fixpoint tsl_rec1' (relTrans: nat -> nat) (E : tsl_table) (t : term) : term :=
   let debug case symbol :=
       debug_term ("tsl_rec1: " ^ case ^ " " ^ symbol ^ " not found") in
   match t with
@@ -46,54 +149,85 @@ Fixpoint tsl_rec1 (E : tsl_table) (t : term) : term :=
   | tSort s => (* s ⇒ λ (A:s). A → s *)
   (* s_1: s -> s' and for A:s, s_1 A holds and A_1 : s_1 A *)
   (* a relation over types A of sort s, the s in the end is the property *)
-    tLambda (nNamed "A") (tSort s) (tProd nAnon (tRel 0) (tSort s))
+    tLambda (nNamed "X") (tSort s) (tProd nAnon (tRel 0) (tSort s))
   | tProd na A B =>
   (* ∀ (x:A). B ⇒ λ(f:∀(x:A_0,B_0)). ∀(x:A_0) (xᵗ:A_1 x). B_1 (f x) *)
   (* the translation relates functions A->B 
     by the relation of their results (B) on related inputs (x) *)
   (* TODO: code *)
-    let A0 := tsl_rec0 0 A in
+
+  (* for A^t take relations like A -> lift up to position of A *)
+  (* for apply to tRel 0 which is A *)
+    (* let A0 := lift0 1 (tsl_rec0' 0 A) in *)
+    let A0 := (tsl_rec0' 0 A) in
+    let A1 := tsl_rec1' relTrans E A in
+    (* let B0 := lift 1 1 (tsl_rec0' 1 B) in *)
+    let B0 := (tsl_rec0' 1 B) in
+    let B1 := tsl_rec1' (up relTrans) E B in
+    let ΠAB0 := tProd na A0 B0 in (* could (maybe) & should be infered *)
+    tLambda (nNamed "f") ΠAB0
+      (tProd na (lift0 1 A0)
+      (*     x  :  A      *)
+                (* lift over f *)
+             (tProd (tsl_name tsl_ident na)
+                    (subst_app (lift0 2 A1) [tRel 0])
+                    (* xᵗ           Aᵗ           x  *)
+                               (* lift over x, f *)
+                    (* (subst_app (lift0 0 (lift 1 2 B1)) *)
+                    (subst_app (lift0 1 (lift 1 2 B1))
+                    (* (subst_app (lift0 1 (lift 0 2 B1)) *)
+                                (* lift after x over f and all over x^t *)
+                               [tApp (tRel 2) [tRel 1]])))
+                               (*       f        x *)
+
+
+    (* let A0 := tsl_rec0 0 A in
     let A1 := tsl_rec1 E A in
     let B0 := tsl_rec0 1 B in
     let B1 := tsl_rec1 E B in
-    let ΠAB0 := tProd na A0 B0 in (* could & should be infered *)
+    let ΠAB0 := tProd na A0 B0 in (* could (maybe) & should be infered *)
     tLambda (nNamed "f") ΠAB0
       (tProd na (lift0 1 A0)
              (tProd (tsl_name tsl_ident na)
                     (subst_app (lift0 2 A1) [tRel 0])
                     (subst_app (lift 1 2 B1)
-                               [tApp (tRel 2) [tRel 1]])))
+                               [tApp (tRel 2) [tRel 1]]))) *)
 
   (* values *)
+  (* | tRel (S k) => (* x ⇒ xᵗ *)
+    tRel k *)
   | tRel k => (* x ⇒ xᵗ *)
   (* TODO: code *)
-  (* 
+  (* TODO: maybe wrong
   Q x, T  -> Q x x^t, T
   0(x) => 0(x^t)
 
   Q y z, T -> Q y y^t z z^t, T
   1(y) => 2(y^t)
   *)
-    tRel (2 * k)
-  | tLambda na A t => 
+    (* tRel k *)
+    tRel k
+    (* tRel (relTrans k) *)
+    (* tRel (2 * k) *)
+  | tLambda na A t =>  (* ignore firt *)
   (* TODO: type of result, code *)
     (* λ(x:A).t ⇒ λ(x:A_0)(xᵗ:A_1 x). t_1 *)
 
     (* proof of function A->B is translated to proof 
       of a relation of B taking related arguments
     *)
-    let A0 := tsl_rec0 0 A in
-    let A1 := tsl_rec1 E A in
+    let A0 := tsl_rec0' 0 A in
+    let A1 := tsl_rec1' relTrans E A in
     tLambda na A0 (tLambda (tsl_name tsl_ident na)
                            (subst_app (lift0 1 A1) [tRel 0])
-                           (tsl_rec1 E t))
+                           (tsl_rec1' relTrans E t))
   | tApp t us =>
   (* t1 t2 ⇒ t1_1 t2_0 t2_1 *)
   (* for every argument t2 the relation of t1 is supplied with
    the argument t2 and the relation over t2 *)
   (* TODO: code *)
-    let us' := concat (map (fun v => [tsl_rec0 0 v; tsl_rec1 E v]) us) in
-    mkApps (tsl_rec1 E t) us'
+    let us' := concat (map (fun v => [tsl_rec0' 0 v; tsl_rec1' relTrans E v]) us) in
+    mkApps (tsl_rec1' relTrans E t) us'
 
   (* | tLetIn na t A u =>
   (* TODO: documentation, code *)
@@ -120,20 +254,18 @@ Fixpoint tsl_rec1 (E : tsl_table) (t : term) : term :=
         lookupConstant, 
         constantRef (t:term) {H:isConstant t}, 
         isConstant *)
+  (* all three constants are translated by a lookup in the table *)
   | tConst s univs =>
-  (* TODO: documentation, code *)
     match lookup_tsl_table E (ConstRef s) with
     | Some t => t
     | None => debug "tConst" (string_of_kername s)
     end
   | tInd i univs =>
-  (* TODO: documentation, code *)
     match lookup_tsl_table E (IndRef i) with
     | Some t => t
     | None => debug "tInd" (match i with mkInd s _ => string_of_kername s end)
     end
   | tConstruct i n univs =>
-  (* TODO: documentation, code *)
     match lookup_tsl_table E (ConstructRef i n) with
     | Some t => t
     | None => debug "tConstruct" (match i with mkInd s _ => string_of_kername s end)
@@ -157,6 +289,27 @@ Fixpoint tsl_rec1 (E : tsl_table) (t : term) : term :=
   | tVar _ | tEvar _ _ => todo "tsl"
   end.
 
+Definition tsl_rec1 := tsl_rec1_app None.
+(* Definition tsl_rec1 := tsl_rec1'. *)
+
+Load de_bruijn_print.
+Definition pretty_print := print_term (empty_ext []) [] true.
+(* Definition test := <% Type %>. *)
+(* Definition test := (tRel 0). *)
+(* Problems *)
+(* Definition test := (tProd nAnon (tRel 0) (tRel 1)). *)
+Definition test := <% forall (A:Type), forall (a:A), Type %>.
+(* Definition test := <% forall (T:Type), Type %>. *)
+Definition testᵗ := tsl_rec1' (fun n => n) [] test.
+Definition testᵗ2 := tsl_rec1 [] test.
+(* Print test.
+Compute testᵗ. *)
+
+MetaCoq Run (print_nf test).
+MetaCoq Run (bruijn_print testᵗ).
+MetaCoq Run (bruijn_print testᵗ2).
+
+Compute (pretty_print (testᵗ)).
 
 
 
@@ -294,7 +447,7 @@ Definition tsl_ident' id := tsl_ident(fst(lastPart id)).
 (* registeres the unary parametricity translations as translation instance *)
 Instance param : Translation :=
   {| tsl_id := tsl_ident' ;
-     tsl_tm := fun ΣE t => ret (tsl_rec1 (snd ΣE) t) ;
+     tsl_tm := fun ΣE t => ret (tsl_rec1' (snd ΣE) t) ;
      (* Implement and Implement Existing cannot be used with this translation *)
      tsl_ty := None ;
      tsl_ind := fun ΣE mp kn mind => 
@@ -323,7 +476,7 @@ Definition checkTranslation (ΣE:tsl_context) (ref:global_reference) : TemplateM
           match opt with (* match over custom option type for inference results *)
           | my_Some x => 
             let Σ' := fst ΣE in
-            let E' := (@content _ x)  ++ (snd ΣE) in (* TODO: can contain duplicates (see below) *)
+            let E' := ((@content _ x)  ++ (snd ΣE))%list in (* TODO: can contain duplicates (see below) *)
             Σ' <- tmEval lazy Σ' ;;
             E' <- tmEval lazy E' ;;
             ret (Σ', E')
